fstar/test/MLS.Test.FromExt.TranscriptHashes.fst
@@ -13,6 +13,7 @@ open MLS.Crypto
 open MLS.TreeDEM.NetworkTypes
 open MLS.TreeDEM.Message.Transcript
 open MLS.TreeDEM.Message.Framing
+open MLS.TreeKEM.KeySchedule
 
 val test_transcript_hashes_one: transcript_hashes_test -> ML bool
 let test_transcript_hashes_one t =
@@ -33,16 +34,16 @@ let test_transcript_hashes_one t =
       let confirmation_key = hex_string_to_bytes t.confirmation_key in
       let interim_transcript_hash_before = hex_string_to_bytes t.interim_transcript_hash_before in
       let confirmed_transcript_hash_after = extract_result (compute_confirmed_transcript_hash authenticated_content.wire_format authenticated_content.content authenticated_content.auth.signature interim_transcript_hash_before) in
-      let confirmation_tag = extract_result (compute_message_confirmation_tag confirmation_key confirmed_transcript_hash_after) in
+      let confirmation_tag = extract_result (compute_confirmation_tag confirmation_key confirmed_transcript_hash_after) in
       let interim_transcript_hash_after = extract_result (compute_interim_transcript_hash #bytes authenticated_content.auth.confirmation_tag confirmed_transcript_hash_after) in
       check_equal "confirmed_transcript_hash_after" (bytes_to_hex_string) (hex_string_to_bytes t.confirmed_transcript_hash_after) (confirmed_transcript_hash_after);
       check_equal "interim_transcript_hash_after" (bytes_to_hex_string) (hex_string_to_bytes t.interim_transcript_hash_after) (interim_transcript_hash_after);
 
       if not (authenticated_content.content.content.content_type = CT_commit) then
         failwith "test_transcript_hashes_one: not a commit"
-      else if not (extract_result (check_authenticated_content_confirmation_tag authenticated_content confirmation_key confirmed_transcript_hash_after)) then
-        failwith "test_transcript_hashes_one: bad confirmation_tag"
-      ;
+      else (
+        check_equal "confirmation_tag" (bytes_to_hex_string) (authenticated_content.auth.confirmation_tag) (confirmation_tag)
+      );
       true
     )
   end
