fstar/treekem/code/MLS.TreeKEM.API.KeySchedule.fst
@@ -10,14 +10,15 @@ open MLS.Result
 
 val create_from_epoch_secret:
   #bytes:Type0 -> {|crypto_bytes bytes|} ->
-  bytes ->
+  bytes -> group_context_nt bytes ->
   result (treekem_keyschedule_state bytes & bytes)
-let create_from_epoch_secret #bytes #cb epoch_secret =
+let create_from_epoch_secret #bytes #cb epoch_secret group_context =
   let? sender_data_secret = secret_epoch_to_sender_data epoch_secret in
   let? encryption_secret = secret_epoch_to_encryption epoch_secret in
   let? exporter_secret = secret_epoch_to_exporter epoch_secret in
   let? external_secret = secret_epoch_to_external epoch_secret in
   let? confirmation_key = secret_epoch_to_confirmation epoch_secret in
+  let? confirmation_tag = compute_confirmation_tag (confirmation_key <: bytes) group_context.confirmed_transcript_hash in
   let? membership_key = secret_epoch_to_membership epoch_secret in
   let? resumption_psk = secret_epoch_to_resumption epoch_secret in
   let? epoch_authenticator = secret_epoch_to_authentication epoch_secret in
@@ -27,10 +28,10 @@ let create_from_epoch_secret #bytes #cb epoch_secret =
       sender_data_secret;
       exporter_secret;
       external_secret;
-      confirmation_key;
       membership_key;
       resumption_psk;
       epoch_authenticator;
+      confirmation_tag;
     };
     init_secret;
   } <: treekem_keyschedule_state bytes), (encryption_secret <: bytes))
@@ -41,7 +42,7 @@ val create_from_joiner_secret:
   result (treekem_keyschedule_state bytes & bytes)
 let create_from_joiner_secret #bytes #cb joiner_secret psks group_context =
   let? epoch_secret = secret_joiner_to_epoch joiner_secret psks group_context in
-  create_from_epoch_secret (epoch_secret <: bytes)
+  create_from_epoch_secret (epoch_secret <: bytes) group_context
 
 type secrets_for_welcome (bytes:Type0) = {
   joiner_secret: bytes;
@@ -59,7 +60,7 @@ let commit #bytes #cb st opt_commit_secret psks new_group_context =
   let? joiner_secret: bytes = secret_init_to_joiner st.init_secret opt_commit_secret new_group_context in
   let? epoch_secret: bytes = secret_joiner_to_epoch joiner_secret psks new_group_context in
   let? welcome_secret: bytes = secret_joiner_to_welcome joiner_secret psks in
-  let? (new_st, encryption_secret) = create_from_epoch_secret epoch_secret in
+  let? (new_st, encryption_secret) = create_from_epoch_secret epoch_secret new_group_context in
   return (new_st, encryption_secret, {
     joiner_secret;
     welcome_secret;
